---
title: Negative triangle inequality
layout: default
---
We prove this the same way we prove the normal triangle inequality, using the identity $Re(x\overline{y}) \leq 2|x||\overline{y}$:
$$ \begin{aligned}
|x - y|^2 &= (x - y)\overline{(x - y)} \\\\
         &= |x|^2 - x\overline{y} - \overline{y}x + |y|^2 \\\\
         &= |x|^2 + |y|^2 - 2\Re(x\overline{y}) \\\\
         \geq |x|^2 + |y|^2 - 2|x||y|
         = (|x| - |y|)^2
\end{aligned} $$
the conclusion follows from taking the square roots of both sides.

